Rename Ifte_free_write/ifte_zip/fuse'/fuse

Minimp/FuseIfte.v
@@ -225,32 +225,32 @@ Proof.
       apply Iifte_false with (1:=Hs2) (2:=Ht2).
 Qed.
 
-Inductive Ifte_free_write : stmt -> Prop :=
+Inductive Is_fusible : stmt -> Prop :=
 | IFWAssign: forall x e,
-    Ifte_free_write (Assign x e)
+    Is_fusible (Assign x e)
 | IFWAssignSt: forall x e,
-    Ifte_free_write (AssignSt x e)
+    Is_fusible (AssignSt x e)
 | IFWIfte: forall e s1 s2,
-    Ifte_free_write s1 ->
-    Ifte_free_write s2 ->
+    Is_fusible s1 ->
+    Is_fusible s2 ->
     (forall x, Is_free_in_exp x e -> ~Can_write_in x s1 /\ ~Can_write_in x s2) ->
-    Ifte_free_write (Ifte e s1 s2)
+    Is_fusible (Ifte e s1 s2)
 | IFWStep_ap: forall x cls obj e,
-    Ifte_free_write (Step_ap x cls obj e)
+    Is_fusible (Step_ap x cls obj e)
 | IFWComp: forall s1 s2,
-    Ifte_free_write s1 ->
-    Ifte_free_write s2 ->
-    Ifte_free_write (Comp s1 s2)
+    Is_fusible s1 ->
+    Is_fusible s2 ->
+    Is_fusible (Comp s1 s2)
 | IFWSkip:
-    Ifte_free_write Skip.
+    Is_fusible Skip.
 
-Lemma lift_Ifte_free_write:
+Lemma lift_Is_fusible:
   forall e s1 s2 t1 t2,
-    Ifte_free_write (Comp (Ifte e s1 s2) (Ifte e t1 t2))
+    Is_fusible (Comp (Ifte e s1 s2) (Ifte e t1 t2))
     <->
-    Ifte_free_write (Ifte e (Comp s1 t1) (Comp s2 t2)).
+    Is_fusible (Ifte e (Comp s1 t1) (Comp s2 t2)).
 Proof.
-  Hint Constructors Ifte_free_write.
+  Hint Constructors Is_fusible.
   intros e s1 s2 t1 t2.
   split; intro Hifw.
   - inversion_clear Hifw as [| | | |? ? Hs Ht|].
@@ -264,21 +264,21 @@ Require Import List.
 Import List.ListNotations.
 Open Scope list_scope.
 
-Lemma Ifte_free_write_fold_left_shift:
+Lemma Is_fusible_fold_left_shift:
   forall A f (xs : list A) iacc,
-    Ifte_free_write (fold_left (fun i x => Comp (f x) i) xs iacc)
+    Is_fusible (fold_left (fun i x => Comp (f x) i) xs iacc)
     <->
-    (Ifte_free_write (fold_left (fun i x => Comp (f x) i) xs Skip)
-     /\ Ifte_free_write iacc).
+    (Is_fusible (fold_left (fun i x => Comp (f x) i) xs Skip)
+     /\ Is_fusible iacc).
 Proof.
-  Hint Constructors Ifte_free_write.
+  Hint Constructors Is_fusible.
   induction xs as [|x xs IH]; [now intuition|].
   intros; split.
   - intro HH. simpl in HH. apply IH in HH.
     destruct HH as [Hxs Hiacc].
     split; [simpl; rewrite IH|];
     repeat progress match goal with
-    | H:Ifte_free_write (Comp _ _) |- _ => inversion_clear H
+    | H:Is_fusible (Comp _ _) |- _ => inversion_clear H
     | _ => now intuition
     end.
   - intros [HH0 HH1].
@@ -286,13 +286,13 @@ Proof.
     simpl; rewrite IH.
     intuition.
     repeat progress match goal with
-    | H:Ifte_free_write (Comp _ _) |- _ => inversion_clear H
+    | H:Is_fusible (Comp _ _) |- _ => inversion_clear H
     | _ => now intuition
     end.
 Qed.
 
 (*
-   The property "Ifte_free_write (translate_eqns mems eqs)" is obtained above
+   The property "Is_fusible (translate_eqns mems eqs)" is obtained above
    using scheduling assumptions for EqDef, since they are needed to treat
    the translation of merge expressions, and clocking assumptions for EqApp and
    EqFby. While the EqApp case can also be obtained from the scheduling
@@ -308,7 +308,7 @@ Qed.
       if x { mem(x) = y }
 
    This program is well scheduled, but it does not satisfy the invariant
-   Ifte_free_write. We could imagine a weaker invariant that allows the
+   Is_fusible. We could imagine a weaker invariant that allows the
    right-most write under an expression to change free variables in the
    expression, which suffices to justify the optimisation, but the
    preservation of this invariant under the optimisation likely becomes much
@@ -321,22 +321,22 @@ Qed.
    are effectively always present).
  *)
 
-Fixpoint ifte_zip s1 s2 : stmt :=
+Fixpoint zip s1 s2 : stmt :=
   match s1, s2 with
   | Ifte e1 t1 f1, Ifte e2 t2 f2 =>
       if exp_eqb e1 e2
-      then Ifte e1 (ifte_zip t1 t2) (ifte_zip f1 f2)
+      then Ifte e1 (zip t1 t2) (zip f1 f2)
       else Comp s1 s2
   | Skip, s => s
   | s,    Skip => s
-  | Comp s1' s2', _ => Comp s1' (ifte_zip s2' s2)
+  | Comp s1' s2', _ => Comp s1' (zip s2' s2)
   | s1,   s2 => Comp s1 s2
   end.
 
-Lemma Can_write_in_ifte_zip:
+Lemma Can_write_in_zip:
   forall s1 s2 x,
     (Can_write_in x s1 \/ Can_write_in x s2)
-    <-> Can_write_in x (ifte_zip s1 s2).
+    <-> Can_write_in x (zip s1 s2).
 Proof.
   Hint Constructors Can_write_in.
   induction s1, s2; simpl;
@@ -352,32 +352,32 @@ Proof.
            | |- Can_write_in _ (Ifte _ _ _) =>
              (apply CWIIfteTrue; apply IHs1_1; now intuition)
              || (apply CWIIfteFalse; apply IHs1_2; now intuition)
-           | H:Can_write_in _ (ifte_zip _ _) |- _ =>
+           | H:Can_write_in _ (zip _ _) |- _ =>
              apply IHs1_1 in H || apply IHs1_2 in H
-           | |- Can_write_in _ (Comp _ (ifte_zip _ _)) =>
+           | |- Can_write_in _ (Comp _ (zip _ _)) =>
              now (apply CWIComp2; apply IHs1_2; intuition)
            | _ => intuition
            end.
 Qed.
 
-Lemma Cannot_write_in_ifte_zip:
+Lemma Cannot_write_in_zip:
   forall s1 s2 x,
     (~Can_write_in x s1 /\ ~Can_write_in x s2)
-    <-> ~Can_write_in x (ifte_zip s1 s2).
+    <-> ~Can_write_in x (zip s1 s2).
 Proof.
   intros s1 s2 x.
   split; intro HH.
-  - intro Hcan; apply Can_write_in_ifte_zip in Hcan; intuition.
-  - split; intro Hcan; apply HH; apply Can_write_in_ifte_zip; intuition.
+  - intro Hcan; apply Can_write_in_zip in Hcan; intuition.
+  - split; intro Hcan; apply HH; apply Can_write_in_zip; intuition.
 Qed.
 
-Lemma ifte_zip_free_write:
+Lemma zip_free_write:
   forall s1 s2,
-    Ifte_free_write s1
-    -> Ifte_free_write s2
-    -> Ifte_free_write (ifte_zip s1 s2).
+    Is_fusible s1
+    -> Is_fusible s2
+    -> Is_fusible (zip s1 s2).
 Proof.
-  Hint Constructors Ifte_free_write Can_write_in.
+  Hint Constructors Is_fusible Can_write_in.
   induction s1, s2;
     intros Hfree1 Hfree2;
     inversion_clear Hfree1;
@@ -391,10 +391,10 @@ Proof.
   constructor;
     repeat progress
            match goal with
-           | H1:Ifte_free_write ?s1,
-             H2:Ifte_free_write ?s2,
-             Hi:context [Ifte_free_write (ifte_zip _ _)]
-             |- Ifte_free_write (ifte_zip ?s1 ?s2)
+           | H1:Is_fusible ?s1,
+             H2:Is_fusible ?s2,
+             Hi:context [Is_fusible (zip _ _)]
+             |- Is_fusible (zip ?s1 ?s2)
              => apply Hi with (1:=H1) (2:=H2)
            | |- forall x, Is_free_in_exp x ?e -> _
              => intros x Hfree
@@ -402,16 +402,16 @@ Proof.
                 H2:Is_free_in_exp _ ?e |- _
              => specialize (H1 _ H2)
            | |- _ /\ _ => split
-           | |- ~Can_write_in _ (ifte_zip _ _)
-             => apply Cannot_write_in_ifte_zip; intuition
+           | |- ~Can_write_in _ (zip _ _)
+             => apply Cannot_write_in_zip; intuition
            | _ => idtac
            end.
 Qed.
 
-Lemma ifte_zip_Comp':
+Lemma zip_Comp':
   forall s1 s2,
-    Ifte_free_write s1
-    -> (stmt_eval_eq (ifte_zip s1 s2) (Comp s1 s2)).
+    Is_fusible s1
+    -> (stmt_eval_eq (zip s1 s2) (Comp s1 s2)).
 Proof.
   induction s1, s2;
   try rewrite stmt_eval_eq_Comp_Skip1;
@@ -424,9 +424,9 @@ Proof.
          | |- context [exp_eqb ?e1 ?e2]
            => destruct (exp_eqb e1 e2) eqn:Heq;
              [apply exp_eqb_eq in Heq; subst|]
-         | H:Ifte_free_write ?s1,
-             IH:context [stmt_eval_eq (ifte_zip ?s1 _) _]
-           |- context [ifte_zip ?s1 ?s2]
+         | H:Is_fusible ?s1,
+             IH:context [stmt_eval_eq (zip ?s1 _) _]
+           |- context [zip ?s1 ?s2]
            => rewrite IH with (1:=H)
          end;
   try (rewrite lift_Ifte; [|assumption]);
@@ -434,212 +434,212 @@ Proof.
   reflexivity.
 Qed.
 
-Fixpoint ifte_fuse' s1 s2 : stmt :=
+Fixpoint fuse' s1 s2 : stmt :=
   match s1, s2 with
-  | s1, Comp s2 s3 => ifte_fuse' (ifte_zip s1 s2) s3
-  | s1, s2 => ifte_zip s1 s2
+  | s1, Comp s2 s3 => fuse' (zip s1 s2) s3
+  | s1, s2 => zip s1 s2
   end.
 (*
-NB: almost got rid of ifte_zip, but this function decreases on the first
-    argument, whereas the remaining instance of ifte_zip requires a decrease
+NB: almost got rid of zip, but this function decreases on the first
+    argument, whereas the remaining instance of zip requires a decrease
     on the second argument...
-Fixpoint ifte_fuse' s1 s2 : stmt :=
+Fixpoint fuse' s1 s2 : stmt :=
   match s1, s2 with
   | Ifte e1 t1 f1, Ifte e2 t2 f2 =>
       if exp_eqb e1 e2
-      then Ifte e1 (ifte_fuse' t1 t2) (ifte_fuse' f1 f2)
+      then Ifte e1 (fuse' t1 t2) (fuse' f1 f2)
       else Comp s1 s2
-  | s1, Comp s2 s3 => ifte_fuse' (ifte_fuse' s1 s2) s3
+  | s1, Comp s2 s3 => fuse' (fuse' s1 s2) s3
   | Skip, s => s
   | s,    Skip => s
-  | Comp s1' s2', Ifte _ _ _ => Comp s1' (ifte_zip s2' s2)
+  | Comp s1' s2', Ifte _ _ _ => Comp s1' (zip s2' s2)
   | s1,   s2 => Comp s1 s2
   end.
 *)
 
-Definition ifte_fuse s : stmt :=
+Definition fuse s : stmt :=
   match s with
-  | Comp s1 s2 => ifte_fuse' s1 s2
+  | Comp s1 s2 => fuse' s1 s2
   | _ => s
   end.
 
-Lemma ifte_fuse'_free_write:
+Lemma fuse'_free_write:
   forall s2 s1,
-    Ifte_free_write s1
-    -> Ifte_free_write s2
-    -> Ifte_free_write (ifte_fuse' s1 s2).
+    Is_fusible s1
+    -> Is_fusible s2
+    -> Is_fusible (fuse' s1 s2).
 Proof.
   induction s2;
-    try (intros; apply ifte_zip_free_write; assumption).
+    try (intros; apply zip_free_write; assumption).
   intros s1 Hfree1 Hfree2.
   inversion_clear Hfree2.
   apply IHs2_2; [|assumption].
-  apply ifte_zip_free_write; assumption.
+  apply zip_free_write; assumption.
 Qed.
 
-(** ifte_eval_eq *)
+(** fuse_eval_eq *)
 
 Require Import Relations.
 Require Import Morphisms.
 Require Import Setoid.
 
-Definition ifte_eval_eq s1 s2: Prop :=
-  stmt_eval_eq s1 s2 /\ (Ifte_free_write s1 /\ Ifte_free_write s2).
+Definition fuse_eval_eq s1 s2: Prop :=
+  stmt_eval_eq s1 s2 /\ (Is_fusible s1 /\ Is_fusible s2).
 
 (*
 Print relation.
-Check (ifte_eval_eq : relation stmt).
+Check (fuse_eval_eq : relation stmt).
  *)
 
-Lemma ifte_eval_eq_refl:
+Lemma fuse_eval_eq_refl:
   forall s,
-    Ifte_free_write s
-    -> Proper ifte_eval_eq s.
+    Is_fusible s
+    -> Proper fuse_eval_eq s.
 Proof.
-  intros s Hfree; unfold Proper, ifte_eval_eq; intuition.
+  intros s Hfree; unfold Proper, fuse_eval_eq; intuition.
 Qed.
 
-Lemma ifte_eval_eq_trans:
-  transitive stmt ifte_eval_eq.
+Lemma fuse_eval_eq_trans:
+  transitive stmt fuse_eval_eq.
 Proof.
   intros s1 s2 s3 Heq1 Heq2.
-  unfold ifte_eval_eq in *.
+  unfold fuse_eval_eq in *.
   split; [|now intuition].
   destruct Heq1 as [Heq1 ?].
   destruct Heq2 as [Heq2 ?].
   rewrite Heq1, Heq2; reflexivity.
 Qed.
 
-Lemma ifte_eval_eq_sym:
-  symmetric stmt ifte_eval_eq.
+Lemma fuse_eval_eq_sym:
+  symmetric stmt fuse_eval_eq.
 Proof.
   intros s1 s2 Heq.
-  unfold ifte_eval_eq in *.
+  unfold fuse_eval_eq in *.
   split; [|now intuition].
   destruct Heq as [Heq ?].
   rewrite Heq; reflexivity.
 Qed.
 
-Add Relation stmt (ifte_eval_eq)
-    symmetry proved by ifte_eval_eq_sym
-    transitivity proved by ifte_eval_eq_trans
-  as ifte_eval_equiv.
+Add Relation stmt (fuse_eval_eq)
+    symmetry proved by fuse_eval_eq_sym
+    transitivity proved by fuse_eval_eq_trans
+  as fuse_eval_equiv.
 
-Instance subrelation_stmt_ifte_eval_eq:
-  subrelation ifte_eval_eq stmt_eval_eq.
+Instance subrelation_stmt_fuse_eval_eq:
+  subrelation fuse_eval_eq stmt_eval_eq.
 Proof.
   intros s1 s2 Heq x menv env menv' env'.
   now apply Heq.
 Qed.
 
-Lemma ifte_zip_Comp:
+Lemma zip_Comp:
   forall s1 s2,
-    Ifte_free_write s1
-    -> Ifte_free_write s2
-    -> ifte_eval_eq (ifte_zip s1 s2) (Comp s1 s2).
+    Is_fusible s1
+    -> Is_fusible s2
+    -> fuse_eval_eq (zip s1 s2) (Comp s1 s2).
 Proof.
   intros s1 s2 Hfree1 Hfree2.
-  unfold ifte_eval_eq.
+  unfold fuse_eval_eq.
   split; [|split].
-  - rewrite ifte_zip_Comp' with (1:=Hfree1); reflexivity.
-  - apply ifte_zip_free_write with (1:=Hfree1) (2:=Hfree2).
+  - rewrite zip_Comp' with (1:=Hfree1); reflexivity.
+  - apply zip_free_write with (1:=Hfree1) (2:=Hfree2).
   - intuition.
 Qed.
 
 (* TODO: Why don't we get this automatically via the subrelation? *)
-Instance ifte_eval_eq_Proper:
-    Proper (eq ==> eq ==> eq ==> ifte_eval_eq ==> eq ==> iff) stmt_eval.
+Instance fuse_eval_eq_Proper:
+    Proper (eq ==> eq ==> eq ==> fuse_eval_eq ==> eq ==> iff) stmt_eval.
 Proof.
   intros prog' prog HR1 menv' menv HR2 env' env HR3 s1 s2 Heq r' r HR4;
   subst; destruct r as [menv' env'].
-  unfold ifte_eval_eq in Heq.
+  unfold fuse_eval_eq in Heq.
   destruct Heq as [Heq ?].
   rewrite Heq; reflexivity.
 Qed.
 
-Instance ifte_eval_eq_Comp_Proper:
-  Proper (ifte_eval_eq ==> ifte_eval_eq ==> ifte_eval_eq) Comp.
+Instance fuse_eval_eq_Comp_Proper:
+  Proper (fuse_eval_eq ==> fuse_eval_eq ==> fuse_eval_eq) Comp.
 Proof.
-  Hint Constructors Ifte_free_write.
+  Hint Constructors Is_fusible.
   intros s s' Hseq t t' Hteq.
-  unfold ifte_eval_eq in *.
+  unfold fuse_eval_eq in *.
   destruct Hseq as [Hseq [Hfrees Hfrees']].
   destruct Hteq as [Hteq [Hfreet Hfreet']].
   split; [|intuition].
   rewrite Hseq, Hteq; reflexivity.
 Qed.
 
-Instance ifte_zip_ifte_eval_eq_Proper:
-  Proper (ifte_eval_eq ==> ifte_eval_eq ==> ifte_eval_eq) ifte_zip.
+Instance zip_fuse_eval_eq_Proper:
+  Proper (fuse_eval_eq ==> fuse_eval_eq ==> fuse_eval_eq) zip.
 Proof.
   intros s s' Hseq t t' Hteq.
-  unfold ifte_eval_eq in *.
+  unfold fuse_eval_eq in *.
   destruct Hseq as [Hseq [Hfrees Hfrees']].
   destruct Hteq as [Hteq [Hfreet Hfreet']].
-  split; [|split]; [|apply ifte_zip_free_write with (1:=Hfrees) (2:=Hfreet)
-                    |apply ifte_zip_free_write with (1:=Hfrees') (2:=Hfreet')].
-  rewrite ifte_zip_Comp' with (1:=Hfrees).
-  rewrite ifte_zip_Comp' with (1:=Hfrees').
+  split; [|split]; [|apply zip_free_write with (1:=Hfrees) (2:=Hfreet)
+                    |apply zip_free_write with (1:=Hfrees') (2:=Hfreet')].
+  rewrite zip_Comp' with (1:=Hfrees).
+  rewrite zip_Comp' with (1:=Hfrees').
   rewrite Hseq, Hteq; reflexivity.
 Qed.
 
-Lemma ifte_fuse'_Comp:
+Lemma fuse'_Comp:
   forall s2 s1,
-    Ifte_free_write s1
-    -> Ifte_free_write s2
-    -> stmt_eval_eq (ifte_fuse' s1 s2) (Comp s1 s2).
+    Is_fusible s1
+    -> Is_fusible s2
+    -> stmt_eval_eq (fuse' s1 s2) (Comp s1 s2).
 Proof.
-  Hint Constructors Ifte_free_write.
+  Hint Constructors Is_fusible.
   induction s2;
   intros s1 Hifte1 Hifte2; simpl;
-  try now (rewrite ifte_zip_Comp'; intuition).
+  try now (rewrite zip_Comp'; intuition).
   rewrite Comp_assoc.
   inversion_clear Hifte2.
   rewrite IHs2_2;
     match goal with
-    | H1:Ifte_free_write ?s1,
-      H2:Ifte_free_write ?s2 |- Ifte_free_write (ifte_zip ?s1 ?s2)
-      => apply ifte_zip_free_write with (1:=H1) (2:=H2)
-    | |- Ifte_free_write ?s => assumption
-    | H:Ifte_free_write s2_2 |- _ => pose proof (ifte_eval_eq_refl _ H)
+    | H1:Is_fusible ?s1,
+      H2:Is_fusible ?s2 |- Is_fusible (zip ?s1 ?s2)
+      => apply zip_free_write with (1:=H1) (2:=H2)
+    | |- Is_fusible ?s => assumption
+    | H:Is_fusible s2_2 |- _ => pose proof (fuse_eval_eq_refl _ H)
     end.
   intros prog menv env menv' env'.
-  rewrite ifte_zip_Comp; [now apply iff_refl|assumption|assumption].
+  rewrite zip_Comp; [now apply iff_refl|assumption|assumption].
 Qed.
 
-Instance ifte_fuse'_ifte_eval_eq_Proper:
-  Proper (ifte_eval_eq ==> ifte_eval_eq ==> ifte_eval_eq) ifte_fuse'.
+Instance fuse'_fuse_eval_eq_Proper:
+  Proper (fuse_eval_eq ==> fuse_eval_eq ==> fuse_eval_eq) fuse'.
 Proof.
   intros s s' Hseq t t' Hteq.
-  unfold ifte_eval_eq in *.
+  unfold fuse_eval_eq in *.
   destruct Hseq as [Hseq [Hfrees Hfrees']].
   destruct Hteq as [Hteq [Hfreet Hfreet']].
-  split; [|split]; [|apply ifte_fuse'_free_write with (1:=Hfrees) (2:=Hfreet)
-                    |apply ifte_fuse'_free_write with (1:=Hfrees') (2:=Hfreet')].
-  repeat rewrite ifte_fuse'_Comp; try assumption.
+  split; [|split]; [|apply fuse'_free_write with (1:=Hfrees) (2:=Hfreet)
+                    |apply fuse'_free_write with (1:=Hfrees') (2:=Hfreet')].
+  repeat rewrite fuse'_Comp; try assumption.
   rewrite Hseq, Hteq.
   reflexivity.
 Qed.
 
-Lemma ifte_fuse_Comp:
+Lemma fuse_Comp:
   forall s,
-    Ifte_free_write s
-    -> stmt_eval_eq (ifte_fuse s) s.
+    Is_fusible s
+    -> stmt_eval_eq (fuse s) s.
 Proof.
   intros s Hfree prog menv env menv' env'.
   destruct s; simpl; try reflexivity.
   inversion_clear Hfree.
   destruct s2;
   match goal with
-  | H: Ifte_free_write ?s2 |- context [ifte_fuse' _ ?s2]
-    => pose proof (ifte_eval_eq_refl _ H)
+  | H: Is_fusible ?s2 |- context [fuse' _ ?s2]
+    => pose proof (fuse_eval_eq_refl _ H)
   end;
-  rewrite ifte_fuse'_Comp; auto; reflexivity.
+  rewrite fuse'_Comp; auto; reflexivity.
 Qed.
 
 (*
 Open Scope positive_scope.
-Eval cbv in (ifte_fuse (Comp (Ifte (Var 1) (Assign 2 (Const (Cint 7))) Skip)
+Eval cbv in (fuse (Comp (Ifte (Var 1) (Assign 2 (Const (Cint 7))) Skip)
                              (Comp (Ifte (Var 1) (Assign 4 (Var 2))
                                          (Assign 4 (State 3)))
                                    (Comp (Ifte (Var 1) Skip
